commit

AP/AP/DisjA.lean
@@ -137,6 +137,87 @@ theorem State.aHwsDisj_insert_of_mem_taken {s fsp p} [hs : sys.WF s]
 (h₁ : s.aHwsDisj fsp) (h₂ : p ∈ s.taken) : s.aHwsDisj (fsp.insert 0 p) := by
   obtain ⟨a, ha, h₁⟩ := h₁; use a, ha, aForallWinsDisj_insert_of_mem_taken h₁ h₂
 
+theorem State.aWinsDisj_of_aWinsDisj_offset {s : State} {st : Strat} {fsp : FSP} {n}
+(h : s.aWinsDisj (fsp.offset n) st) : s.aWinsDisj fsp st := by
+  intro k; specialize h k; obtain ⟨s₁, h₁, h₂⟩ := h; use s₁, h₁
+  simp at h₂; contrapose! h₂; exact fsp.hasLe_of_add_right h₂
+
+theorem State.aForallWinsDisj_of_aForallWinsDisj_offset {s : State} {a : AStrat}
+{fsp : FSP} {n} (h : s.aForallWinsDisj (fsp.offset n) a) : s.aForallWinsDisj fsp a :=
+  λ d hd => aWinsDisj_of_aWinsDisj_offset # h d hd
+
+theorem State.aHwsDisj_of_aHwsDisj_offset {s : State} {fsp : FSP} {n}
+(h : s.aHwsDisj (fsp.offset n)) : s.aHwsDisj fsp := by
+  obtain ⟨a, ha, h⟩ := h; use a, ha, aForallWinsDisj_of_aForallWinsDisj_offset h
+
+theorem State.aWinsDisj_of_aWinsDisj_next {s : State} {st : Strat} {fsp : FSP}
+(h : s.aWinsDisj fsp.next st) : s.aWinsDisj fsp st :=
+  aWinsDisj_of_aWinsDisj_offset (n := 1) h
+
+theorem State.aForallWinsDisj_of_aForallWinsDisj_next {s : State} {a : AStrat}
+{fsp : FSP} (h : s.aForallWinsDisj fsp.next a) : s.aForallWinsDisj fsp a :=
+  aForallWinsDisj_of_aForallWinsDisj_offset (n := 1) h
+
+theorem State.aHwsDisj_of_aHwsDisj_next {s : State} {fsp : FSP}
+(h : s.aHwsDisj fsp.next) : s.aHwsDisj fsp :=
+  aHwsDisj_of_aHwsDisj_offset (n := 1) h
+
+-- #check 0 #exit
+
+theorem State.aHwsDisj_setHist_of_aHwsDisj {s fsp hist} [hs : sys.WF s]
+[hs' : sys.WF # s.setHist hist] (h : s.aHwsDisj fsp) : (s.setHist hist).aHwsDisj fsp := by
+  obtain ⟨a, ha, h⟩ := h
+  use .mk # λ sa => a.f # sa.setHistAt s.hist hist
+  use inferInstance
+  intro d hd n
+  specialize h # .mk # λ sd' => d.f # sd'.setHistAt hist s.hist
+  specialize h inferInstance n
+  obtain ⟨s₁, h₁, h₂⟩ := h
+  use s₁.setHistAt s.hist hist
+  constructor
+  · sorry
+  · sorry
+
+-- #check 0 #exit
+
+@[simp]
+theorem State.aHwsDisj_setHist_iff {s fsp hist} [hs : sys.WF s]
+[hs' : sys.WF # s.setHist hist] : (s.setHist hist).aHwsDisj fsp ↔ s.aHwsDisj fsp := by
+  symm; use aHwsDisj_setHist_of_aHwsDisj
+  intro h; change s.setHist hist |>.setHist s.hist |>.aHwsDisj fsp
+  exact aHwsDisj_setHist_of_aHwsDisj h
+
+-- #check 0 #exit
+
+def aDisjEraseTaken (s₀ s₀' : State) (p₀ : PointZ) (a : AStrat) : AStrat :=
+  .mkFold (α := State × PointZ × AStrat) s₀' ⟨s₀, p₀, a⟩
+  (λ _ ⟨s, p, a⟩ => ⟨a.f s, sys.tr s (a.f s) |>.get!, p, a⟩) #
+  λ _ p₁ ⟨s, p, a⟩ =>
+    if p₁ ≠ p then ⟨sys.tr s p₁ |>.get!, p, a⟩ else
+    ⟨sys.tr s s.chooseDMove |>.get!, s.chooseDMove, a⟩
+
+@[simp]
+instance {s₀ s₀' p₀ a} : (aDisjEraseTaken s₀ s₀' p₀ a).WF := by
+  unfold aDisjEraseTaken; infer_instance
+
+-- #check 0 #exit
+
+theorem State.aHwsDisj_erase_taken {fsp s s' p} [hs : sys.WF s] [hs' : sys.WF s']
+(h : s.aHwsDisj fsp) (hpw : s'.pw = s.pw) (ht : s'.aTurn = s.aTurn)
+(hpa : s'.aPos = s.aPos) (hp : s'.taken = s.taken.erase p) : s'.aHwsDisj fsp := by
+  by_cases h₁ : p ∉ s.taken
+  · rw [Set'.erase_eq_of_not_mem h₁] at hp
+    have h₂ : s' = s.setHist s'.hist
+    · ext:1 <;> first | assumption | simp
+    rw [h₂] at hs' ⊢ ;exact aHwsDisj_setHist_of_aHwsDisj h
+  push_neg at h₁
+  obtain ⟨a, ha, h⟩ := h
+  use aDisjEraseTaken s s' p a, inferInstance
+  intro d hd n
+  sorry
+
+-- #check 0 #exit
+
 theorem AState.aHwsDisj_nbhd_pw {s : State} {fsp : FSP} [hs : AState s]
 (h : s.aHwsDisj fsp) : s.aHwsDisj # fsp.insertSet 3 # s.aPos.nbhd s.pw |>.toSet := by
   sorry
